theories/adequacy.v
@@ -23,6 +23,7 @@ Section proofs.
   (* Helping the inference with this notation that hides Δ *)
   Local Notation "s <: t" := (@subtype _ s t) (at level 70, no associativity).
   Local Notation "lty <:< rty" := (@lty_sub _ lty rty) (at level 70, no associativity).
+  Local Notation "lts <: vs :> rts" := (@subtype_targs _ vs lts rts) (at level 70, vs at next level).
 
   (* heap models relation; the semantic heap does
      not appear because it is hidden in iProp  *)
@@ -45,15 +46,17 @@ Section proofs.
     map_Forall (λ _cname, wf_cdef_fields) Δ →
     map_Forall (λ _cname, wf_cdef_fields_bounded) Δ →
     map_Forall (λ _cname, wf_cdef_parent Δ) Δ →
+    map_Forall (λ _ : string, wf_cdef_mono) Δ →
+    map_Forall (λ _, wf_ty) lty →
     expr_eval le e = Some val →
     expr_has_ty lty e ty →
     interp_local_tys σi lty le -∗
     interp_type ty σi val.
   Proof.
-    move => ??? he h; move: le val he.
+    move => ????? he h; move: le val he.
     elim: h => [z | b | | op e1 e2 hop he1 hi1 he2 hi2 |
         op e1 e2 hop he1 hi1 he2 hi2 |
-        v vty hv | exp S T hS hi hwf hsub ] =>  le val he; iIntros "#Hlty".
+        v vty hv | exp S T hS hi hwf hsub ] => le val he; iIntros "#Hlty".
     - inv he; rewrite interp_type_unfold /=; by eauto.
     - inv he; rewrite interp_type_unfold /=; by eauto.
     - inv he; rewrite interp_type_unfold /=; by eauto.
@@ -94,7 +97,8 @@ Section proofs.
       rewrite H0 in H; by case: H => ->.
     - apply hi in he.
       iApply subtype_is_inclusion => //.
-      by iApply he.
+      + by apply expr_has_ty_wf in hS.
+      + by iApply he.
   Qed.
 
   Lemma interp_local_tys_update σi v lty le ty val :
@@ -113,6 +117,8 @@ Section proofs.
     map_Forall (λ _cname, wf_cdef_fields) Δ →
     map_Forall (λ _cname, wf_cdef_fields_bounded) Δ →
     map_Forall (λ _cname, wf_cdef_parent Δ) Δ →
+    map_Forall (λ _ : string, wf_cdef_mono) Δ →
+    map_Forall (λ _, wf_ty) lty →
     dom stringset targs = dom stringset args →
     map_args (expr_eval le) args = Some vargs →
     (∀ (x : string) (ty : lang_ty) (arg : expr),
@@ -122,7 +128,7 @@ Section proofs.
     interp_local_tys σi lty le -∗
     interp_local_tys σi targs vargs.
   Proof.
-    move => ??? hdom hargs helt.
+    move => ????? hdom hargs helt.
     iIntros "#Hle" (v ty) "%hin".
     assert (ha: ∃ arg, args !! v = Some arg).
     { apply elem_of_dom.
@@ -145,25 +151,30 @@ Section proofs.
     by iApply expr_adequacy.
   Qed.
 
-  Lemma heap_models_update h l rt vs σi t σt f fty v:
+  Lemma heap_models_update h l rt vs (σi: interp_env) t σt f fty v:
     map_Forall (λ _cname, wf_cdef_parent Δ) Δ →
     map_Forall (λ _cname, wf_cdef_fields) Δ →
     map_Forall (λ _cname, wf_cdef_fields_bounded) Δ →
+    map_Forall (λ _ : string, wf_cdef_fields_wf) Δ →
+    (* Note: overkill, contra is enough for fields in this proof *)
+    map_Forall (λ _cname, wf_field_mono) Δ →
+    map_Forall (λ _ : string, wf_cdef_mono) Δ →
     h !! l = Some (rt, vs) →
     has_field f t fty →
+    wf_ty (ClassT t σt) →
     interp_type (ClassT t σt) σi (LocV l) -∗
     interp_type (subst_ty σt fty) σi v -∗
     heap_models h -∗
     heap_models (<[l:=(rt, <[f:=v]> vs)]> h).
   Proof.
-    move => ?? hfb hheap hfield.
+    move => ?? hfb ??? hheap hfield hwf.
     iIntros "#hrecv #hv hmodels".
     iDestruct "hmodels" as (sh) "[hown [%hdom #h]]".
     iExists sh.
     rewrite interp_class_unfold.
-    iDestruct "hrecv" as (l' t' σ' σt' fields ifields) "[%H [hsem hl]]".
+    iDestruct "hrecv" as (l' t' def σ' σt' fields ifields) "[%H [hsem hl]]".
     iDestruct "hsem" as "[%hdomf #hifields]".
-    destruct H as [[= <-] [ hinherits' [hwfσ' [hσ' hfields]]]].
+    destruct H as [[= <-] [ hinherits' [hwfσ' [hdef [hσ' hfields]]]]].
     iDestruct (sem_heap_own_valid_2 with "hown hl") as "#Hv".
     iSplitL; first by iFrame.
     iSplitR.
@@ -202,13 +213,33 @@ Section proofs.
           iNext.
           iSpecialize ("hf'" $! v).
           iRewrite -"hf'".
-          rewrite subst_ty_subst //.
-          apply has_field_bounded in hfield => //.
-          destruct hfield as (def & hdef & hfty).
-          apply inherits_using_wf in hinherits' => //.
-          destruct hinherits' as (? & ? & ? & ? & _ & hL & _).
-          simplify_eq.
-          by rewrite hL.
+          rewrite subst_ty_subst; last first.
+          { apply has_field_bounded in hfield => //.
+            destruct hfield as (def' & hdef' & hfty).
+            apply inherits_using_wf in hinherits' => //.
+            destruct hinherits' as (? & ? & ? & ? & _ & hL & _).
+            simplify_eq.
+            by rewrite hL.
+          }
+          assert (hsub : subst_ty σt fty <: subst_ty (subst_ty σt' <$> σ') fty).
+          { clear hdom hdomf hdomv.
+            assert (hfwf := hfield).
+            apply has_field_wf in hfwf => //.
+            apply has_field_mono in hfield => //.
+            destruct hfield as (tdef & ? & [_ hcontra]); simplify_eq.
+            apply subtype_lift with (neg_variance <$> generics tdef) => //.
+            - by apply wf_ty_class_inv in hwf.
+            - apply wf_ty_subst_map.
+              + by apply wf_ty_class_inv in hwfσ'.
+              + apply inherits_using_wf in hinherits' => //.
+                by repeat destruct hinherits' as [? hinherits'].
+            - by apply neg_subtype_targs.
+
+          }
+          iApply subtype_is_inclusion => //.
+          apply has_field_wf in hfield => //.
+          apply wf_ty_subst => //.
+          by apply wf_ty_class_inv in hwf.
         * rewrite lookup_insert_ne //.
           by iApply "hmodfs".
     - iApply "h".
@@ -231,7 +262,7 @@ Section proofs.
         lty lhs recv t targs name fty hrecv hf |
         lty recv fld rhs fty t σ hrecv hrhs hf |
         lty lhs t targs args fields hwf hf hdom harg |
-        lty lhs recv t targs name orig mdef args hrecv hfrom hdom hi |
+        lty lhs recv t targs name orig mdef args hrecv hhasm hdom hi |
         lty c rty' rty hsub h hi |
         lty rty v tv t cmd hv hr h hi
       ] "IHty" forall (st st' n hc).
@@ -262,8 +293,8 @@ Section proofs.
       iModIntro. (* keep the later *)
       iDestruct (expr_adequacy with "Hle") as "#He" => //; try (by apply wfΔ).
       rewrite interp_class_unfold /=.
-      iDestruct "He" as (??????) "[%H [#Hifields H◯]]".
-      destruct H as [[= <-] [hinherits [_ [htargs hfields]]]].
+      iDestruct "He" as (???????) "[%H [#Hifields H◯]]".
+      destruct H as [[= <-] [hinherits [hwfσt [hdef [htargs hfields]]]]].
       iAssert (heap_models h ∗ ▷ interp_type (subst_ty targs fty) σi v)%I with "[Hh]" as "[Hh Hv]".
       { iDestruct "Hh" as (sh) "(H● & %hdom & #Hh)".
         iDestruct (sem_heap_own_valid_2 with "H● H◯") as "#HΦ".
@@ -284,7 +315,28 @@ Section proofs.
         iRewrite -"HΦ" in "Hifields_t".
         iSpecialize ("h" $! name _ with "[Hifields_t]"); first done.
         iDestruct "h" as (w) "[%hw hiw]".
-        by simplify_eq.
+        iNext.
+        destruct wfΔ.
+        assert (hsub: subst_ty (subst_ty σt <$> σ) fty <: subst_ty targs fty).
+        { clear hdom hdiom hdf.
+          assert (hfwf := hf).
+          apply has_field_wf in hfwf => //.
+          apply has_field_mono in hf => //.
+          destruct hf as (tdef & ? & [hcov _]); simplify_eq.
+          apply subtype_lift with (generics tdef) => //.
+          - apply wf_ty_subst_map; first by apply wf_ty_class_inv in hwfσt.
+            apply inherits_using_wf in hinherits => //.
+            by repeat destruct hinherits as [? hinherits].
+          - apply expr_has_ty_wf in hrecv => //.
+            by apply wf_ty_class_inv in hrecv.
+        }
+        simplify_eq.
+        iApply subtype_is_inclusion => //.
+        apply wf_ty_subst.
+        * apply wf_ty_subst_map; first by apply wf_ty_class_inv in hwfσt.
+          apply inherits_using_wf in hinherits => //.
+          by repeat destruct hinherits as [? hinherits].
+        * by apply has_field_wf in hf.
       }
       iNext.
       iFrame.
@@ -295,6 +347,7 @@ Section proofs.
       iClear "IH".
       iIntros "[Hh #Hle]" => /=.
       iSplitL; last done.
+      assert (ht: wf_ty (ClassT t σ)) by (by apply expr_has_ty_wf in hrecv).
       iApply heap_models_update => //.
       + iApply expr_adequacy => //; by apply wfΔ.
       + iApply expr_adequacy => //; by apply wfΔ.
@@ -324,12 +377,13 @@ Section proofs.
         rewrite interp_type_unfold /=.
         assert (hwf' := hwf).
         inv hwf'.
-        iExists new, t, (gen_targs def.(generics)), targs, fields, iFs.
+        iExists new, t, def, (gen_targs (length def.(generics))), targs, fields, iFs.
         iSplit; last by (repeat iSplit => //).
         iPureIntro.
         repeat split => //.
         + by econstructor.
-        + by rewrite subst_ty_gen_targs.
+        + rewrite subst_ty_gen_targs => //.
+          by apply subtype_targs_refl.
       }
       iSplitL; last by iApply interp_local_tys_update.
       iExists _. iFrame. iSplit; first by rewrite !dom_insert_L Hdom.
@@ -387,10 +441,19 @@ Section proofs.
       destruct wfΔ.
       (* Get inherits relation between dynamic tag and static tag *)
       iIntros "[Hh #Hle]".
+      (* make the script more resilient. Should provide a proper inversion
+       * lemma but this is the next best thing.
+       *)
+      rename H3 into heval_recv.
+      rename H4 into hmap.
+      rename H5 into hheap.
+      rename H7 into hhasm0.
+      rename H11 into heval_body.
+      rename H12 into heval_ret.
       iDestruct (expr_adequacy _ recv with "Hle") as "#Hrecv" => //.
       rewrite interp_class_unfold /=.
-      iDestruct "Hrecv" as (? ? σin σt fields ifields) "[%Hpure [hifields Hl]]".
-      destruct Hpure as [[= <-] [hσin [hwfσt [htargs hfields]]]].
+      iDestruct "Hrecv" as (? t1 def σin σt fields ifields) "[%Hpure [hifields Hl]]".
+      destruct Hpure as [[= <-] [hin_t1_t [hwf_t1_σt [hdef [htargs hfields]]]]].
       iDestruct "Hh" as (sh) "(H● & %Hdom & #Hh)".
       iDestruct (sem_heap_own_valid_2 with "H● Hl") as "#HΦ".
       iDestruct ("Hh" with "[//]") as (?) "[H H▷]".
@@ -400,84 +463,85 @@ Section proofs.
       fold_leibniz; subst.
       (* both static and dynamic classes actually exists in Δ *)
       assert (ht1: is_Some (Δ !! t1)).
-      { apply has_method_from_def in H7 as (? & ? & ? & ? & _ & [? [hin ?]]) => //.
+      { apply has_method_from_def in hhasm0 as (? & ? & ? & ? & _ & [? [hin ?]]) => //.
         by apply inherits_using_wf in hin as (? & ? & ht1 & _).
       }
-      assert (ht : is_Some (Δ !! t)).
-      { apply inherits_using_wf in hσin => //.
-        by destruct hσin as (? & ? & _ & -> & _).
-      }
-      destruct ht as [ def ht ].
-      destruct ht1 as [ def1 ht1 ].
+      destruct ht1 as [ def1 hdef1 ].
       (* Get method inclusion information between mdef0 and mdef *)
       destruct (has_method_ordered _ _ _ _ _ _ _ _
         wf_extends_wf wf_override wf_parent wf_methods_bounded
-        hσin H7 hfrom)
-      as (σmin & σot1 & σot & odef0 & odef & omdef0 & omdef &
-         hσeq & ho1 & ho & hom1 & hom & hino & hin1 & hin &
-         _ & ? & heq0 & heq1 & hincl0 & hincl1).
+        hin_t1_t hhasm0 hhasm)
+      as (σoin & σot1 & σot & odef0 & odef & omdef0 & omdef &
+         hσeq & hodef0 & hodef & homdef0 & homdef & hin_o_o0 & hin_t1_o0 & hin_t_o &
+         _ & _ & -> & -> & hincl0 & hincl1).
       (* Get location of the definition of the dynamic method mdef0 *)
-      destruct (has_method_from_def _ _ _ _  wf_parent wf_methods_bounded H7) as
-        (odef0' & mdef0_orig & ho0 & hm0 & hmorig0 & [σ0 [hin0 ->]]).
-      rewrite ho0 in ho1; injection ho1; intros; subst; clear ho1.
-      rewrite subst_mdef_body in H11.
-      rewrite subst_mdef_ret in H12.
+      destruct (has_method_from_def _ _ _ _  wf_parent wf_methods_bounded hhasm0) as
+        (odef0' & mdef0_orig & hodef0' & hmdef0_orig & hhasm_morig0 & [σ0 [hin_t1_o0' heqmdef]]).
+      rewrite hodef0 in hodef0'; injection hodef0'; intros <-; clear hodef0'.
+      rewrite homdef0 in hmdef0_orig; injection hmdef0_orig; intros <-; clear hmdef0_orig.
+      replace σot1 with σ0 in *; last by eapply inherits_using_fun.
+      clear σot1 hin_t1_o0' heqmdef.
+      rewrite subst_mdef_body in heval_body.
+      rewrite subst_mdef_ret in heval_ret.
       (* Get some type info about dynamic method mdef0 *)
-      assert (hwf0 := hin0).
+      assert (hwf0 := hin_t1_o0).
       eapply wf_mdef_ty_inherits in hwf0 => //; last first.
-      { apply wf_mdefs in ho0.
-        by apply ho0 in hm0.
+      { apply wf_mdefs in hodef0.
+        by apply hodef0 in homdef0.
       }
       (* Random helpers statements *)
-      assert (bounded (length σ0) (methodrettype mdef0_orig)).
-      { assert (ho0' := ho0).
-        apply wf_methods_bounded in ho0'.
-        apply ho0' in hm0.
-        destruct hm0 as [_ hret].
-        apply inherits_using_wf in hin0 => //.
-        repeat destruct hin0 as [? hin0]; simplify_eq.
-        by rewrite H6.
+      assert (hb_ret0: bounded (length σ0) (methodrettype omdef0)).
+      { assert (h0 := hodef0).
+        apply wf_methods_bounded in h0.
+        apply h0 in homdef0.
+        destruct homdef0 as [_ hret].
+        apply inherits_using_wf in hin_t1_o0 => //.
+        destruct hin_t1_o0 as (? & ? & ? & ? & ? & hL &?); simplify_eq.
+        by rewrite hL.
       }
-      assert (map_Forall (λ _ : string, bounded (length σ0)) (methodargs mdef0_orig)).
-      { assert (ho0' := ho0).
-        apply wf_methods_bounded in ho0'.
-        apply ho0' in hm0.
-        destruct hm0 as [hargs _].
+      assert (hb_a0 : map_Forall (λ _ : string, bounded (length σ0)) (methodargs omdef0)).
+      { assert (h0 := hodef0).
+        apply wf_methods_bounded in h0.
+        apply h0 in homdef0.
+        destruct homdef0 as [hargs _].
         rewrite map_Forall_lookup => k tk hk.
         apply hargs in hk.
-        apply inherits_using_wf in hin0 => //.
-        repeat destruct hin0 as [? hin0]; simplify_eq.
-        by rewrite H8.
+        apply inherits_using_wf in hin_t1_o0 => //.
+        destruct hin_t1_o0 as (? & ? & ? & ? & ? & hL &?); simplify_eq.
+        by rewrite hL.
       }
-      assert (map_Forall (λ _ : string, bounded (length σot)) (methodargs omdef)).
-      { assert (ho' := ho).
-        apply wf_methods_bounded in ho'.
-        apply ho' in hom.
-        destruct hom as [hargs _].
+      assert (hb_ao: map_Forall (λ _ : string, bounded (length σot)) (methodargs omdef)).
+      { assert (h0 := hodef).
+        apply wf_methods_bounded in h0.
+        apply h0 in homdef.
+        destruct homdef as [hargs _].
         rewrite map_Forall_lookup => k tk hk.
         apply hargs in hk.
-        apply inherits_using_wf in hin => //.
-        repeat destruct hin as [? hin]; simplify_eq.
-        by rewrite H9.
+        apply inherits_using_wf in hin_t_o => //.
+        destruct hin_t_o as (? & ? & ? & ? & ? & hL &?); simplify_eq.
+        by rewrite hL.
       }
-      assert (length σt = generics def1).
-      { inv hwfσt.
+      assert (hl0: length σt = length (generics def1)).
+      { inv hwf_t1_σt.
         by simplify_eq.
       }
-      assert (Forall wf_ty σt) by (by apply wf_ty_class_inv in hwfσt).
-      assert (hwfot1: Forall wf_ty σot1).
-      { apply inherits_using_wf in hin1 => //.
-        by repeat destruct hin1 as [? hin1].
+      assert (hwf_σt: Forall wf_ty σt) by (by apply wf_ty_class_inv in hwf_t1_σt).
+      assert (hwfσot1: Forall wf_ty σ0).
+      { apply inherits_using_wf in hin_t1_o0 => //.
+        by repeat destruct hin_t1_o0 as [? hin_t1_o0].
       }
       (* specialize the typing judgement of the method by adding the
        * runtime type substitution.
        *)
-      assert (hwf1: wf_mdef_ty (ClassT t1 σt) (subst_ty σt <$> σ0) mdef0_orig).
-      { destruct hwf0 as [rty0 [hbody0 hret0]].
-        exists (subst_ty σt <$> rty0); split; last first.
-        + rewrite -subst_ty_subst //.
-          by apply expr_has_ty_subst.
-        + replace (ClassT t1 σt) with (subst_ty σt (ClassT t1 (gen_targs (generics def1)))); last first.
+      assert (hwf1: wf_mdef_ty (ClassT t1 σt) (subst_ty σt <$> σ0) omdef0).
+      { destruct hwf0 as [rty0 [wf0 [hbody0 hret0]]].
+        exists (subst_ty σt <$> rty0); split; last split.
+        + rewrite map_Forall_lookup => k ty.
+          rewrite lookup_fmap_Some.
+          case => [ty' [<- hk]].
+          apply wf_ty_subst => //.
+          by apply wf0 in hk.
+        + replace (ClassT t1 σt) with (subst_ty σt (ClassT t1 (gen_targs (length (generics def1))))); last first.
           { simpl.
             by rewrite subst_ty_gen_targs.
           }
@@ -491,53 +555,63 @@ Section proofs.
           * rewrite lookup_fmap_Some.
             case => [tx [<- hk]].
             apply wf_ty_subst.
-            { apply inherits_using_wf in hin0 => //.
-              by repeat destruct hin0 as [? hin0].
-            }
-            apply has_method_wf in hmorig0 as [hargs _] => //.
+            { by apply inherits_using_wf in hin_t1_o0. }
+            apply has_method_wf in hhasm_morig0 as [hargs _] => //.
             by apply hargs in hk.
+        + rewrite -subst_ty_subst //.
+          by apply expr_has_ty_subst.
       }
-      destruct hwf1 as [rty1 [hbody1 hret1]].
+      destruct hwf1 as [rty1 [wf1 [hbody1 hret1]]].
       (* manual clean up *)
-      rewrite hm0 in hom1; injection hom1; intros; subst; clear hom1.
-      replace σ0 with σot1 in *; last by eapply inherits_using_fun.
-      clear hin0.
       assert (wfbody:
         map_Forall (λ _ : string, wf_ty)
-          (<["$this":=ClassT t1 σt]> (subst_ty (subst_ty σt <$> σot1) <$> methodargs omdef0))
+          (<["$this":=ClassT t1 σt]> (subst_ty (subst_ty σt <$> σ0) <$> methodargs omdef0))
       ).
       { rewrite map_Forall_lookup => x tx.
         rewrite lookup_insert_Some.
         case => [[? <-]|[?]] => //.
         rewrite lookup_fmap_Some.
         case => [tx' [ <- hx]].
-        apply wf_ty_subst.
-        - apply Forall_forall => tk hk.
-          apply elem_of_list_fmap_2 in hk as [tk2 [-> hk]].
-          apply wf_ty_subst => //.
-          rewrite Forall_forall in hwfot1.
-          by apply hwfot1 in hk.
-        - assert (ho0' := ho0).
-          apply wf_methods_wf in ho0'.
-          apply ho0' in hm0.
-          by apply hm0 in hx.
+        apply wf_ty_subst; first by apply wf_ty_subst_map.
+        assert (h0 := hodef0).
+        apply wf_methods_wf in h0.
+        apply h0 in homdef0.
+        by apply homdef0 in hx.
+      }
+      assert (hwf_σin: Forall wf_ty σin).
+      { apply inherits_using_wf in hin_t1_t => //.
+        by repeat destruct hin_t1_t as [? hin_t1_t].
+      }
+      assert (hwf_σt_σin: Forall wf_ty (subst_ty σt <$> σin)) by (by apply wf_ty_subst_map).
+      assert (hwf_targs: Forall wf_ty targs).
+      { apply expr_has_ty_wf in hrecv => //.
+        by apply wf_ty_class_inv in hrecv.
+      }
+      assert (hb_σin_σot : Forall (bounded (length σin)) σot).
+      { apply inherits_using_wf in hin_t1_t => //.
+        destruct hin_t1_t as (? & ? & ? & ? & hF & hL & hwf).
+        apply inherits_using_wf in hin_t_o => //.
+        destruct hin_t_o as (? & ? & ? & ? & hF' & hL' & hwf').
+        simplify_eq.
+        by rewrite hL.
       }
       (* Time ot use the induction hypothesis *)
       iModIntro; iNext.
-      iSpecialize ("IH" $! _ _ _ wfbody hbody1 σi _ _ _ H11); simpl.
+      iSpecialize ("IH" $! _ _ _ wfbody hbody1 σi _ _ _ heval_body); simpl.
       iDestruct ("IH" with "[Hh Hle H●]") as "Hstep".
       { iSplit.
         - iExists _; iFrame.
-          iSplit; first by rewrite Hdom.
-          done.
+          iSplit; last done.
+          by rewrite Hdom.
         - iApply interp_local_tys_update => //; last first.
             + rewrite interp_class_unfold /interp_class /=.
-              iExists l, t1, (gen_targs def1.(generics)), σt, fields, ifields; iSplitR.
+              iExists l, t1, def1, (gen_targs (length def1.(generics))), σt, fields, ifields; iSplitR.
               { iPureIntro; repeat split => //; first by econstructor.
-                by rewrite subst_ty_gen_targs.
+                rewrite subst_ty_gen_targs //.
+                by apply subtype_targs_refl.
               }
               by iSplit.
-            + iApply interp_local_tys_list => //.
+            + iApply (interp_local_tys_list _ lty le) => //.
               * destruct hincl0 as [hdomincl _].
                 rewrite !dom_fmap_L in hdomincl.
                 rewrite !dom_fmap_L in hdom.
@@ -548,45 +622,75 @@ Section proofs.
                 destruct hincl1 as [hdom1 [hincl1 _]].
                 destruct (methodargs omdef !! x) as [ty' | ] eqn:hty'.
                 { assert (bounded (length σot) ty').
-                  { assert (ho' := ho).
-                    apply wf_methods_bounded in ho'.
-                    apply ho' in hom.
-                    apply hom in hty'.
-                    apply inherits_using_wf in hin => //.
-                    destruct hin as ( ? & ? & ? & ? & _ & hL & _); simplify_eq.
+                  { assert (ho := hodef).
+                    apply wf_methods_bounded in ho.
+                    apply ho in homdef.
+                    apply homdef in hty'.
+                    apply inherits_using_wf in hin_t_o => //.
+                    destruct hin_t_o as ( ? & ? & ? & ? & _ & hL & _); simplify_eq.
                     by rewrite hL.
                   }
                   eapply ESubTy.
                   - apply hi with x => //.
                     by rewrite /subst_mdef /= lookup_fmap hty'.
-                  - apply wf_ty_subst.
-                    + rewrite Forall_forall => tk hk.
-                      apply elem_of_list_fmap_2 in hk as [tk2 [-> hk]].
-                      apply wf_ty_subst => //.
-                      rewrite Forall_forall in hwfot1; by apply hwfot1.
-                    + apply has_method_wf in hmorig0 as [hargs _] => //.
-                      by apply hargs in hx.
-                  - rewrite -!subst_ty_subst; first last.
-                    + apply bounded_subst with (length σot) => //.
-                      apply inherits_using_wf in hin => //.
-                      destruct hin as (? & ? & ? & ? & hF & _ & _).
-                      apply inherits_using_wf in hσin => //.
-                      destruct hσin as (? & ? & ? & ? & _ & hL' & _).
+                  - apply wf_ty_subst; first by apply wf_ty_subst_map.
+                    apply has_method_wf in hhasm_morig0 as [hargs _] => //.
+                    by apply hargs in hx.
+                  - (* step by step, using variance info *)
+                    assert (hsub: subst_ty targs (subst_ty σot ty') <: subst_ty (subst_ty σt <$> σin) (subst_ty σot ty')).
+                    { apply subtype_lift with (neg_variance <$> generics def) => //.
+                      - assert (hmono := hodef).
+                        apply wf_methods_mono in hmono.
+                        assert (ho := homdef).
+                        apply hmono in ho as [hmonoa _].
+                        assert (ha := hty').
+                        apply hmonoa in ha.
+                        apply mono_subst with (neg_variance <$> generics odef) => //.
+                        + rewrite map_length.
+                          apply wf_methods_bounded in hodef.
+                          apply hodef in homdef.
+                          by apply homdef in hty'.
+                        + rewrite map_length.
+                          apply inherits_using_wf in hin_t_o => //.
+                          repeat destruct hin_t_o as [? hin_t_o]; by simplify_eq.
+                        + rewrite neg_variance_fmap_idem => i vi ti hvi.
+                          apply list_lookup_fmap_inv in hvi.
+                          destruct hvi as [wi [-> hwi]].
+                          move => hti hc.
+                          apply inherits_using_mono with (def0 := def) in hin_t_o => //.
+                          inv hin_t_o; simplify_eq.
+                          destruct wi; by eauto.
+                        + move => i vi ti hvi.
+                          apply list_lookup_fmap_inv in hvi.
+                          destruct hvi as [wi [-> hwi]].
+                          move => hti hc.
+                          apply inherits_using_mono with (def0 := def) in hin_t_o => //.
+                          inv hin_t_o; simplify_eq.
+                          destruct wi; by eauto.
+                      - apply wf_ty_subst => //.
+                        * apply inherits_using_wf in hin_t_o => //.
+                          by repeat destruct hin_t_o as [? hin_t_o].
+                        * apply wf_methods_wf in hodef.
+                          apply hodef in homdef.
+                          by apply homdef in hty'.
+                      - by apply neg_subtype_targs.
+                    }
+                    eapply SubTrans; first by exact hsub.
+                    rewrite -!subst_ty_subst; first last.
+                    { by apply bounded_subst with (length σot). }
+                    { assert (h0 := hodef0).
+                      apply wf_methods_bounded in h0.
+                      apply h0 in homdef0.
+                      apply homdef0 in hx.
+                      apply inherits_using_wf in hin_t1_o0 => //.
+                      destruct hin_t1_o0 as (? & ? &? &? & ? &hL & ?).
                       simplify_eq.
-                      by rewrite hL'.
-                    + assert (ho0' := ho0).
-                      apply wf_methods_bounded in ho0'.
-                      apply ho0' in hm0.
-                      apply hm0 in hx.
-                      apply inherits_using_wf in hin1 => //.
-                      destruct hin1 as (? & ? & ? & ? & ? & hL' & _).
-                      simplify_eq.
-                      by rewrite hL'.
-                    + apply subtype_subst => //.
-                      rewrite subst_ty_subst //.
-                      apply hincl1 with x => //; first by rewrite /subst_mdef /= lookup_fmap hx.
-                      rewrite /subst_mdef /= fmap_subst_ty_subst //.
-                      by rewrite lookup_fmap hty'.
+                      by rewrite hL.
+                    }
+                    apply subtype_subst => //.
+                    eapply hincl1 with x.
+                    * by rewrite /subst_mdef /= lookup_fmap hx /=.
+                    * by rewrite /subst_mdef /= !lookup_fmap hty' /=.
                 }
                 rewrite /subst_mdef /= !dom_fmap_L in hdom1.
                 apply mk_is_Some in hx.
@@ -601,29 +705,51 @@ Section proofs.
       iIntros "[Hmodels Hle2]"; iFrame.
       iApply interp_local_tys_update; first by done.
       destruct hincl1 as [? [? hret]].
+      assert (hsub: subst_ty (subst_ty σt <$> σ0) (methodrettype omdef0) <:
+                    subst_ty targs (subst_ty σot (methodrettype omdef))).
+      { eapply SubTrans; last first.
+        - apply subtype_lift with (σ1 := subst_ty σt <$> σin) (vs0 := generics def) => //.
+          + assert (hmono := hodef).
+            apply wf_methods_mono in hmono.
+            assert (hm := homdef).
+            apply hmono in hm as [_ hmonoret].
+            apply mono_subst with (generics odef) => //.
+            * apply wf_methods_bounded in hodef.
+              apply hodef in homdef.
+              by apply homdef.
+            * apply inherits_using_wf in hin_t_o => //.
+              repeat destruct hin_t_o as [? hin_t_o]; by simplify_eq.
+            * move => i vi ti hvi hti hc.
+              apply inherits_using_mono with (def0 := def) in hin_t_o => //.
+              inv hin_t_o; simplify_eq.
+              by eauto.
+            * move => i vi ti hvi hti hc.
+              apply inherits_using_mono with (def0 := def) in hin_t_o => //.
+              inv hin_t_o; simplify_eq.
+              by eauto.
+          + apply wf_ty_subst => //.
+            * apply inherits_using_wf in hin_t_o => //.
+              by repeat destruct hin_t_o as [? hin_t_o].
+            * apply wf_methods_wf in hodef.
+              apply hodef in homdef.
+              by apply homdef.
+        - rewrite -!subst_ty_subst //; first by apply subtype_subst.
+          apply bounded_subst with (length σot) => //.
+          apply inherits_using_wf in hin_t_o => //.
+          destruct hin_t_o as (? & ? & ? & ? & ? & hL & _).
+          simplify_eq.
+          assert (ho := hodef).
+          apply wf_methods_bounded in ho.
+          apply ho in homdef.
+          rewrite hL.
+          by apply homdef.
+      }
       iDestruct (expr_adequacy _ (methodret omdef0) with "Hle2") as "#Hret" => //.
-      rewrite -subst_ty_subst; last first.
-      { assert (ho' := ho).
-        apply wf_methods_bounded in ho'.
-        apply ho' in hom.
-        by apply inherits_using_wf in hin.
-      }
-      rewrite -subst_ty_subst; last first.
-      { apply inherits_using_wf in hin => //.
-        destruct hin as ( ? & ? & ? & ? & hF & hL & _).
-        apply inherits_using_wf in hσin => //.
-        destruct hσin as (? & ? & ? & ? & hF' & hL' & _).
-        simplify_eq.
-        apply bounded_subst with odef.(generics) => //; last by rewrite hL'.
-        assert (ho' := ho).
-        apply wf_methods_bounded in ho'.
-        apply ho' in hom.
-        by apply hom.
-      }
-      assert (hsub: subst_ty σt (subst_ty σot1 (methodrettype omdef0)) <:
-                    subst_ty σt (subst_ty σin (subst_ty σot (methodrettype omdef))))
-        by (by apply subtype_subst).
-      by iApply subtype_is_inclusion.
+      iApply subtype_is_inclusion => //.
+      apply wf_ty_subst; first by apply wf_ty_subst_map.
+      apply wf_methods_wf in hodef0.
+      apply hodef0 in homdef0.
+      by apply homdef0.
     - (* Subtyping *) 
       destruct wfΔ.
       iIntros "H".
@@ -631,8 +757,9 @@ Section proofs.
       iApply updN_mono_I; last done.
       iIntros "[Hh #Hrty]". iFrame.
       iDestruct (interp_local_tys_is_inclusion with "Hrty") as "Hrty'" => //.
-      rewrite Forall_forall => i hi v.
-      by apply _.
+      + by apply cmd_has_ty_wf in h.
+      + rewrite Forall_forall => i hi v.
+        by apply _.
     - (* CondTagC *) inv hc; last first.
       { iIntros "[Hh H]".
         iAssert (heap_models st'.2 ∗ interp_local_tys σi rty st'.1)%I with "[Hh H]" as "H".
@@ -661,8 +788,9 @@ Section proofs.
       rewrite Hlev in hl; simplify_eq.
       iAssert (interp_type MixedT σi (LocV l)) as "Hmixed".
       { destruct wfΔ.
-        iApply subtype_is_inclusion; [ done | done | done | by apply SubMixed | ].
-        done.
+        assert (hsub : tv <: MixedT) by apply SubMixed.
+        iApply subtype_is_inclusion => //.
+        by apply wflty in hv.
       }
       rewrite interp_mixed_unfold /=.
       iDestruct "Hmixed" as "[Hnonnull | Hnull]"; last first.
@@ -671,8 +799,9 @@ Section proofs.
       { iDestruct "Hint" as "%Hint"; by destruct Hint. }
       iDestruct "Hl" as "[Hbool | Hl]".
       { iDestruct "Hbool" as "%Hbool"; by destruct Hbool. }
-      iDestruct "Hl" as (exTag exσ k rt σ σt exfields ifields) "[%H [#Hfields #Hl]]".
-      destruct H as [[= <-] [hinherits' [hwf' [ heq' hfields']]]].
+      iDestruct "Hl" as (exTag exσ) "[wfex Hl]".
+      iDestruct "Hl" as (k rt def σ σt exfields ifields) "[%H [#Hfields #Hl]]".
+      destruct H as [[= <-] [hinherits' [hwf' [hdef [ heq' hfields']]]]].
       iAssert (⌜t' = rt⌝ ∗ heap_models st.2 ∗ interp_type (ExT rt) σi (LocV l))%I with "[H]" as "[%heq [Hh #Hv2]]".
       { iDestruct "H" as (sh) "(H● & %hdom & #Hh)".
         iDestruct (sem_heap_own_valid_2 with "H● Hl") as "#HΦ".
@@ -688,14 +817,19 @@ Section proofs.
         { inv hwf'.
           by rewrite H1.
         }
-        destruct hrt as [def hrt].
-        iExists σt, l, rt, (gen_targs def.(generics)), σt, exfields, ifields.
+        destruct hrt as [rdef hrt].
+        iExists σt.
+        iSplitR.
+        { iPureIntro.
+          by apply wf_ty_class_inv in hwf'.
+        }
+        iExists l, rt, rdef, (gen_targs (length rdef.(generics))), σt, exfields, ifields.
         iSplit.
         + iPureIntro; repeat split => //.
           * by constructor.
-          * rewrite subst_ty_gen_targs //.
-            inv hwf'.
-            by simplify_eq.
+          * inv hwf'; simplify_eq.
+            rewrite subst_ty_gen_targs //.
+            by apply subtype_targs_refl.
         + by iSplit.
       }
       subst.
